Added a couple more proofs to EFSM_LTL

theories/EFSM_LTL.thy
@@ -10,8 +10,7 @@ record state =
   event :: event
   "output" :: outputs
 
-type_synonym full_observation = "state stream"
-type_synonym property = "full_observation \<Rightarrow> bool"
+type_synonym property = "state stream \<Rightarrow> bool"
 
 abbreviation label :: "state \<Rightarrow> String.literal" where
   "label s \<equiv> fst (event s)"
@@ -28,20 +27,14 @@ fun ltl_step :: "transition_matrix \<Rightarrow> nat option \<Rightarrow> datast
                      (Some s', (apply_outputs (Outputs t) (join_ir i r)), (apply_updates (Updates t) (join_ir i r) r))
                   )"
 
-primcorec make_full_observation :: "transition_matrix \<Rightarrow> nat option \<Rightarrow> datastate \<Rightarrow> event stream \<Rightarrow> full_observation" where
+primcorec make_full_observation :: "transition_matrix \<Rightarrow> nat option \<Rightarrow> datastate \<Rightarrow> event stream \<Rightarrow> state stream" where
   "make_full_observation e s d i = (let (s', o', d') = ltl_step e s d (shd i) in \<lparr>statename = s, datastate = d, event=(shd i), output = o'\<rparr>##(make_full_observation e s' d' (stl i)))"
 
 lemma make_full_observation_unfold: "make_full_observation e s d i = (let (s', o', d') = ltl_step e s d (shd i) in \<lparr>statename = s, datastate = d, event=(shd i), output = o'\<rparr>##(make_full_observation e s' d' (stl i)))"
   using make_full_observation.code by blast
 
-definition watch :: "transition_matrix \<Rightarrow> event stream \<Rightarrow> full_observation" where
+definition watch :: "transition_matrix \<Rightarrow> event stream \<Rightarrow> state stream" where
   "watch e i \<equiv> (make_full_observation e (Some 0) <> i)"
-
-abbreviation non_null :: "property" where
-  "non_null s \<equiv> (statename (shd s) \<noteq> None)"
-
-abbreviation null :: "property" where
-  "null s \<equiv> (statename (shd s) = None)"
 
 definition Outputs :: "nat \<Rightarrow> state stream \<Rightarrow> value option" where
   "Outputs n s \<equiv> nth (output (shd s)) n"
@@ -61,13 +54,11 @@ definition LabelEq :: "string \<Rightarrow> state stream \<Rightarrow> bool" whe
 lemma watch_label: "LabelEq l (watch e t) = (fst (shd t) = String.implode l)"
   by (simp add: LabelEq_def watch_def)
 
-fun "checkInx" :: "ior \<Rightarrow> nat \<Rightarrow> (value option \<Rightarrow> value option \<Rightarrow> trilean) \<Rightarrow> value option \<Rightarrow> state stream \<Rightarrow> bool" where
-  "checkInx ior.ip n f v s = (f (Some (Inputs (n-1) s)) v = trilean.true)" |
-  "checkInx ior.op n f v s = (f (Outputs n s) v = trilean.true)" |
-  "checkInx ior.rg n f v s = (f (datastate (shd s) (vname.R n)) v = trilean.true)"
-
 definition InputEq :: "value list \<Rightarrow> state stream \<Rightarrow> bool" where
   "InputEq v s \<equiv> inputs (shd s) = v"
+
+definition EventEq :: "(string \<times> inputs) \<Rightarrow> state stream \<Rightarrow> bool" where
+  "EventEq e = LabelEq (fst e) aand InputEq (snd e)"
 
 definition OutputEq :: "value option list \<Rightarrow> state stream \<Rightarrow> bool" where
   "OutputEq v s \<equiv> output (shd s) = v"
@@ -78,21 +69,10 @@ definition InputLength :: "nat \<Rightarrow> state stream \<Rightarrow> bool" wh
 definition OutputLength :: "nat \<Rightarrow> state stream \<Rightarrow> bool" where
   "OutputLength v s \<equiv> length (output (shd s)) = v"
 
-abbreviation some_state :: "full_observation \<Rightarrow> bool" where
-  "some_state s \<equiv> (\<exists>state. statename (shd s) = Some state)"
-
-lemma non_null_equiv: "non_null = some_state"
-  by simp
-
-lemma start_some_state:  "s = make_full_observation e (Some 0) <> t \<Longrightarrow> some_state s"
-  by simp
-
-lemma some_until_none: "s = make_full_observation e (Some 0) <> t \<Longrightarrow> (some_state until null) s "
-proof (coinduction)
-  case UNTIL
-  then show ?case
-    by (smt UNTIL.coinduct non_null_equiv)
-qed
+fun "checkInx" :: "ior \<Rightarrow> nat \<Rightarrow> (value option \<Rightarrow> value option \<Rightarrow> trilean) \<Rightarrow> value option \<Rightarrow> state stream \<Rightarrow> bool" where
+  "checkInx ior.ip n f v s = (f (Some (Inputs (n-1) s)) v = trilean.true)" |
+  "checkInx ior.op n f v s = (f (Outputs n s) v = trilean.true)" |
+  "checkInx ior.rg n f v s = (f (datastate (shd s) (vname.R n)) v = trilean.true)"
 
 lemma shd_state_is_none: "(StateEq None) (make_full_observation e None r t)"
   by (simp add: StateEq_def)
@@ -118,6 +98,24 @@ proof -
     by (simp add: OutputEq_def all_imp_alw)
 qed
 
+lemma no_updates_none: "alw (\<lambda>x. datastate (shd x) = r) (make_full_observation e None r t)"
+proof -
+  obtain ss :: "((String.literal \<times> value list) stream \<Rightarrow> state stream) \<Rightarrow> (String.literal \<times> value list) stream" where
+    "\<forall>f p s. f (stl (ss f)) \<noteq> stl (f (ss f)) \<or> alw p (f s) = alw (\<lambda>s. p (f s)) s"
+    by (metis (no_types) alw_inv)
+  then show ?thesis
+    by (simp add: all_imp_alw)
+qed
+
+lemma no_updates_none_individual: "alw (checkInx rg n ValueEq (r (R n))) (make_full_observation e None r t)"
+proof -
+  obtain ss :: "((String.literal \<times> value list) stream \<Rightarrow> state stream) \<Rightarrow> (String.literal \<times> value list) stream" where
+    "\<forall>f p s. f (stl (ss f)) \<noteq> stl (f (ss f)) \<or> alw p (f s) = alw (\<lambda>s. p (f s)) s"
+    by (metis (no_types) alw_inv)
+  then show ?thesis
+    by (simp add: ValueEq_def all_imp_alw)
+qed
+
 lemma event_components: "(LabelEq l aand InputEq i) s = (event (shd s) = (String.implode l, i))"
   apply (simp add: LabelEq_def InputEq_def)
   by (metis fst_conv prod.collapse snd_conv)
@@ -129,14 +127,5 @@ lemma alw_not_some: "alw (\<lambda>xs. statename (shd xs) \<noteq> Some s) (make
 
 lemma decompose_pair: "e \<noteq> (l, i) = (\<not> (fst e =l \<and> snd e = i))"
   by (metis fst_conv prod.collapse sndI)
-
-lemma check_binding_aand: "(alw x aand y) = (alw x) aand y"
-  by simp
-
-lemma check_binding_or: "(alw x or y) = (alw x) or y"
-  by simp
-
-lemma check_binding_impl: "(alw x impl y) = (alw x) impl y"
-  by simp
 
 end
